

Derivatives

$$\text{Sum: } \frac{d}{dx}(u+v) = \frac{du}{dx} + \frac{dv}{dx}$$

$$\text{Product: } \frac{d}{dx}(uv) = u \frac{dv}{dx} + v \frac{du}{dx}$$

$$\text{Quotient: } \frac{d}{dx}\left(\frac{u}{v}\right) = \frac{v \frac{du}{dx} - u \frac{dv}{dx}}{v^2}$$

$$\text{Power: } \frac{d}{dx}(u^n) = nu^{n-1} \frac{du}{dx}$$

$$\text{Chain: } \frac{d}{dx}z(y(x)) = \frac{dz}{dy} \frac{dy}{dx}$$

$$\text{Inverse: } \frac{dx}{dy} = \frac{1}{dy/dx}$$

$$\frac{d}{dx} \sin x = \cos x$$

$$\frac{d}{dx} \cos x = -\sin x$$

$$\frac{d}{dx} \tan x = \sec^2 x$$

$$\frac{d}{dx} \cot x = -\csc^2 x$$

$$\frac{d}{dx} \sec x = \sec x \tan x$$

$$\frac{d}{dx} \csc x = -\csc x \cot x$$

$$\frac{d}{dx} e^{cx} = ce^{cx}$$

$$\frac{d}{dx} b^x = b^x \ln b$$

$$\frac{d}{dx} \ln x = \frac{1}{x}$$

$$\frac{d}{dx} \sin^{-1} x = \frac{1}{\sqrt{1-x^2}}$$

$$\frac{d}{dx} \tan^{-1} x = \frac{1}{1+x^2}$$

$$\frac{d}{dx} \sec^{-1} x = \frac{1}{|x|\sqrt{x^2-1}}$$

$$\int a^x dx = \frac{1}{\ln a} a^x$$

Limits and Continuity

$$\frac{\sin x}{x} \rightarrow 1 \quad \frac{1-\cos x}{x} \rightarrow 0 \quad \frac{1-\cos x}{x^2} \rightarrow \frac{1}{2}$$

$$a_n \rightarrow 0 : |a_n| < \epsilon \text{ for all } n > N$$

$$a_n \rightarrow L : |a_n - L| < \epsilon \text{ for all } n > N$$

$$f(x) \rightarrow L : |f(x) - L| < \epsilon \text{ for } 0 < |x - a| < \delta$$

$$f(x) \rightarrow f(a) : \text{Continuous at } a \text{ if } L = f(a)$$

$$\frac{f(x)-f(a)}{x-a} \rightarrow f'(a) : \text{Derivative at } a$$

$$\frac{f(x)-f(a)}{x-a} = f'(c) : \text{Mean Value Theorem}$$

$$\frac{f(x+\Delta x)-f(x)}{\Delta x} \rightarrow f'(x) : \text{Derivative at } x$$

$$\frac{f(x+\Delta x)-f(x-\Delta x)}{2\Delta x} \rightarrow f'(x) : \text{Centered}$$

$$\lim_{g(x)} \frac{f(x)}{g(x)} = \lim_{g'(x)} \frac{f'(x)}{g'(x)} \quad \text{l'Hôpital's Rule for } \frac{0}{0}$$

Maximum and Minimum

$$\text{Critical: } f'(x) = 0 \text{ or no } f' \text{ or endpoint}$$

$$\text{Minimum} \quad f'(x) = 0 \text{ and } f''(x) > 0$$

$$\text{Maximum} \quad f'(x) = 0 \text{ and } f''(x) < 0$$

$$\text{Inflection point} \quad f''(x) = 0$$

$$\text{Newton's Method } x_{n+1} = x_n - \frac{f(x_n)}{f'(x_n)}$$

$$\text{Iteration } x_{n+1} = F(x_n) \text{ attracted to fixed point } x^* = F(x^*) \text{ if } |F'(x^*)| < 1$$

$$\text{Stationary in 2D: } \partial f / \partial x = 0, \partial f / \partial y = 0$$

$$\text{Minimum} \quad f_{xx} > 0 \quad f_{xx}f_{yy} > f_{xy}^2$$

$$\text{Maximum} \quad f_{xx} < 0 \quad f_{xx}f_{yy} > f_{xy}^2$$

$$\text{Saddle point} \quad f_{xx}f_{yy} < f_{xy}^2$$

$$\text{Newton in 2D} \begin{cases} g + g_x \Delta x + g_y \Delta y = 0 \\ h + h_x \Delta x + h_y \Delta y = 0 \end{cases}$$

Algebra

$$\frac{x/a}{y/b} = \frac{bx}{ay} \quad x^{-n} = \frac{1}{x^n} \quad \sqrt[n]{x} = x^{1/n}$$

$$(x^2)(x^3) = x^5 \quad (x^2)^3 = x^6 \quad x^2/x^3 = x^{-1}$$

$$ax^2 + bx + c = 0 \text{ has roots } x = \frac{-b \pm \sqrt{b^2 - 4ac}}{2a}$$

$$x^2 + 2Bx + C = 0 \text{ has roots } x = -B \pm \sqrt{B^2 - C}$$

$$\text{Completing square } ax^2 + bx + c = a(x + \frac{b}{2a})^2 + c - \frac{b^2}{4a}$$

$$\text{Partial fractions } \frac{cx+d}{(x-a)(x-b)} = \frac{A}{x-a} + \frac{B}{x-b}$$

$$\text{Mistakes } \frac{a}{b+c} \neq \frac{a}{b} + \frac{a}{c} \quad \sqrt{x^2 + a^2} \neq x + a$$

Fundamental Theorem of Calculus

$$\frac{d}{dx} \int_a^x v(t) dt = v(x) \quad \int_a^b \frac{df}{dx} dx = f(b) - f(a)$$

$$\frac{d}{dx} \int_{a(x)}^{b(x)} v(t) dt = v(b(x)) \frac{db}{dx} - v(a(x)) \frac{da}{dx}$$

$$\int_0^b y(x) dx = \lim_{\Delta x \rightarrow 0} \Delta x [y(\Delta x) + y(2\Delta x) + \dots + y(b)]$$

Circle, Line, and Plane

$$x = r \cos \omega t, y = r \sin \omega t, \text{ speed } \omega r$$

$$y = mx + b \text{ or } y - y_0 = m(x - x_0)$$

$$\text{Plane } ax + by + cz = d \text{ or}$$

$$a(x - x_0) + b(y - y_0) + c(z - z_0) = 0$$

$$\text{Normal vector } ai + bj + ck$$

$$\text{Distance to } (0,0,0): |d|/\sqrt{a^2 + b^2 + c^2}$$

$$\text{Line } (x, y, z) = (x_0, y_0, z_0) + t(v_1, v_2, v_3)$$

$$\text{No parameter: } \frac{x-x_0}{v_1} = \frac{y-y_0}{v_2} = \frac{z-z_0}{v_3}$$

$$\text{Projection: } \mathbf{p} = \frac{\mathbf{b} \cdot \mathbf{a}}{\mathbf{a} \cdot \mathbf{a}} \mathbf{a}, |\mathbf{p}| = |\mathbf{b}| \cos \theta$$

Sums and Infinite Series

$$1 + x + \cdots + x^{n-1} = \frac{1-x^n}{1-x}$$

$$1 + nx + \frac{n(n-1)}{2!}x^2 + \cdots + x^n = (1+x)^n$$

$$1 + 2 + \cdots + n = \frac{1}{2}n(n+1) \approx \frac{n^2}{2}$$

$$1^2 + 2^2 + \cdots + n^2 = \frac{n(n+1)(2n+1)}{6} \approx \frac{n^3}{3}$$

$$1 + \frac{1}{2} + \cdots + \frac{1}{n} \approx \ln n \rightarrow \infty \text{ (harmonic)}$$

$$1 - \frac{1}{2} + \frac{1}{3} - \cdots = \ln 2 \text{ (alternating)}$$

$$1 - \frac{1}{3} + \frac{1}{5} - \cdots = \frac{\pi}{4} \quad \sum \frac{1}{n^2} = \frac{\pi^2}{6} \quad \sum \frac{1}{n^4} = \frac{\pi^4}{90}$$

$$\frac{1}{1-x} = 1 + x + x^2 + \cdots \text{ (geometric: } |x| < 1)$$

$$\frac{1}{(1-x)^2} = 1 + 2x + 3x^2 + \cdots = \frac{d}{dx} \left(\frac{1}{1-x} \right)$$

$$\frac{1}{1+x} = 1 - x + x^2 - \cdots \text{ (geometric for } -x)$$

$$\ln(1+x) = x - \frac{x^2}{2} + \frac{x^3}{3} - \cdots = \int \frac{dx}{1+x}$$

$$\sin x = x - x^3/6 + x^5/120 - \cdots \text{ (all } x)$$

$$\cos x = 1 - x^2/2 + x^4/24 - \cdots \text{ (all } x)$$

$$e^x = 1 + x + \frac{x^2}{2!} + \cdots \text{ (} e = 1 + 1 + \frac{1}{2!} + \cdots)$$

$$e^{ix} = \cos x + i \sin x \text{ (Euler's formula)}$$

$$\cosh x = \frac{1}{2}(e^x + e^{-x}) = 1 + \frac{x^2}{2!} + \cdots$$

$$\sinh x = \frac{1}{2}(e^x - e^{-x}) = x + \frac{x^3}{3!} + \cdots$$

$$(\cos \theta + i \sin \theta)^n = \cos n\theta + i \sin n\theta$$

$$f(x) = f(0) + f'(0)x + \frac{f''(0)}{2!}x^2 + \cdots \text{ (Taylor)}$$

$$f(x, y) = f + x f_x + y f_y + \frac{x^2}{2!} f_{xx} + xy f_{xy} + \cdots$$

Polar and Spherical

$$x = r \cos \theta \text{ and } y = r \sin \theta$$

$$r = \sqrt{x^2 + y^2} \text{ and } \tan \theta = y/x$$

$$x + iy = r(\cos \theta + i \sin \theta) = r e^{i\theta}$$

$$\text{Area } \int \frac{1}{2} r^2 d\theta \quad \text{Length } \int \sqrt{r_\theta^2 + r^2} d\theta$$

$$x = \rho \sin \phi \cos \theta, y = \rho \sin \phi \sin \theta, z = \rho \cos \phi$$

$$\text{Area } dA = dx dy = r dr d\theta = J du dv$$

$$\text{Volume } r dr d\theta dz = \rho^2 \sin \phi d\rho d\phi d\theta$$

$$\text{Stretching factor } J = \frac{\partial(x, y)}{\partial(u, v)} = \begin{vmatrix} x_u & x_v \\ y_u & y_v \end{vmatrix}$$

An additional table of integrals is included just after the index.

Area - Volume - Length - Mass - Moment

$$\text{Circle } \pi r^2 \quad \text{Ellipse } \pi ab \quad \text{Wedge of circle } r^2 \theta / 2$$

$$\text{Cylinder side } 2\pi r h \quad \text{Volume } \pi r^2 h \quad \text{Shell } dV = 2\pi r h dr$$

$$\text{Sphere surface } 4\pi r^2 \quad \text{Volume } \frac{4}{3}\pi r^3 \quad \text{Shell } dV = 4\pi r^2 dr$$

$$\text{Cone or pyramid Volume } \frac{1}{3} (\text{base area}) (\text{height})$$

$$\text{Length of curve } \int ds = \int \sqrt{1 + (dy/dx)^2} dx$$

$$\text{Area between curves } \int (v(x) - w(x)) dx$$

$$\text{Surface area of revolution } \int 2\pi r ds (r = x \text{ or } r = y)$$

$$\text{Volume of revolution: Slices } \int \pi y^2 dx \quad \text{Shells } \int 2\pi x h dx$$

$$\text{Area of surface } z(x, y) : \iint \sqrt{1 + z_x^2 + z_y^2} dx dy$$

$$\text{Mass } M = \iint \rho dA \quad \text{Moment } M_y = \iint \rho x dA$$

$$\bar{x} = M_y/M, \bar{y} = M_x/M \quad \text{Moment of Inertia } I_y = \iint \rho x^2 dA$$

$$\text{Work } W = \int_a^b F(x) dx = V(b) - V(a) \quad \text{Force } F = dV/dx$$

Partial Derivatives of $z = f(x, y)$

$$\text{Tangent plane } z - z_0 = \left(\frac{\partial f}{\partial x}\right)(x - x_0) + \left(\frac{\partial f}{\partial y}\right)(y - y_0)$$

$$\text{Approximation } \Delta z \approx \left(\frac{\partial f}{\partial x}\right)\Delta x + \left(\frac{\partial f}{\partial y}\right)\Delta y$$

$$\text{Normal } \mathbf{N} = (f_x, f_y, -1) \text{ or } (F_x, F_y, F_z)$$

$$\text{Gradient } \nabla f = \frac{\partial f}{\partial x} \mathbf{i} + \frac{\partial f}{\partial y} \mathbf{j}$$

$$\text{Directional derivative: } D_{\mathbf{u}} f = \nabla f \cdot \mathbf{u} = f_x u_1 + f_y u_2$$

$$\text{Chain rule: } \frac{dz}{dt} = \frac{\partial f}{\partial x} \frac{dx}{dt} + \frac{\partial f}{\partial y} \frac{dy}{dt}$$

Vector field $\mathbf{F}(x, y, z) = M \mathbf{i} + N \mathbf{j} + P \mathbf{k}$

$$\text{Work } \int \mathbf{F} \cdot d\mathbf{R} \quad \text{Flux } \int M dy - N dx$$

$$\text{Divergence of } \mathbf{F} = \nabla \cdot \mathbf{F} = \frac{\partial M}{\partial x} + \frac{\partial N}{\partial y} + \frac{\partial P}{\partial z}$$

$$\text{Curl of } \mathbf{F} = \nabla \times \mathbf{F} = \begin{vmatrix} \mathbf{i} & \mathbf{j} & \mathbf{k} \\ \partial/\partial x & \partial/\partial y & \partial/\partial z \\ M & N & P \end{vmatrix}$$

$$\text{Conservative } \mathbf{F} = \nabla f = \text{gradient of } f \text{ if } \text{curl } \mathbf{F} = \mathbf{0}$$

$$\text{Green's Theorem } \oint M dx + N dy = \iint \left(\frac{\partial N}{\partial x} - \frac{\partial M}{\partial y} \right) dx dy$$

$$\text{Divergence Theorem } \iint \mathbf{F} \cdot \mathbf{n} dS = \iiint \text{div } \mathbf{F} dV$$

$$\text{Stokes' Theorem } \oint \mathbf{F} \cdot d\mathbf{R} = \iint (\text{curl } \mathbf{F}) \cdot \mathbf{n} dS$$

Exponentials and Logarithms

$$y = b^x \leftrightarrow x = \log_b y \quad y = e^x \leftrightarrow x = \ln y$$

$$e = \lim(1 + \frac{1}{n})^n = \sum_{n=0}^{\infty} \frac{1}{n!} = 2.71828 \dots$$

$$e^x = \lim(1 + \frac{x}{n})^n = \sum_{n=0}^{\infty} \frac{x^n}{n!}$$

$$\ln y = \int_1^y \frac{dx}{x} \quad \ln 1 = 0 \quad \ln e = 1$$

$$\ln xy = \ln x + \ln y \quad \ln x^n = n \ln x$$

$$\log_a y = (\log_a b)(\log_b y) \quad \log_a b = 1/\log_b a$$

$$e^{x+y} = e^x e^y \quad b^x = e^{x \ln b} \quad e^{\ln y} = y$$

Vectors and Determinants

$$\mathbf{A} = a_1 \mathbf{i} + a_2 \mathbf{j} + a_3 \mathbf{k}$$

$$|\mathbf{A}|^2 = \mathbf{A} \cdot \mathbf{A} = a_1^2 + a_2^2 + a_3^2 \text{ (length squared)}$$

$$\mathbf{A} \cdot \mathbf{B} = a_1 b_1 + a_2 b_2 + a_3 b_3 = |\mathbf{A}| |\mathbf{B}| \cos \theta$$

$$|\mathbf{A} \cdot \mathbf{B}| \leq |\mathbf{A}| |\mathbf{B}| \text{ (Schwarz inequality: } |\cos \theta| \leq 1)$$

$$|\mathbf{A} + \mathbf{B}| \leq |\mathbf{A}| + |\mathbf{B}| \text{ (triangle inequality)}$$

$$|\mathbf{A} \times \mathbf{B}| = |\mathbf{A}| |\mathbf{B}| \sin \theta \text{ (cross product)}$$

$$\mathbf{A} \times \mathbf{B} = \begin{vmatrix} \mathbf{i} & \mathbf{j} & \mathbf{k} \\ a_1 & a_2 & a_3 \\ b_1 & b_2 & b_3 \end{vmatrix} = \begin{vmatrix} i(a_2 b_3 - a_3 b_2) \\ +j(a_3 b_1 - a_1 b_3) \\ +k(a_1 b_2 - a_2 b_1) \end{vmatrix}$$

Right hand rule $\mathbf{i} \times \mathbf{j} = \mathbf{k}$, $\mathbf{j} \times \mathbf{k} = \mathbf{i}$, $\mathbf{k} \times \mathbf{i} = \mathbf{j}$

Parallelogram area $= |a_1 b_2 - a_2 b_1| = |\text{Det}|$

Triangle area $= \frac{1}{2} |a_1 b_2 - a_2 b_1| = \frac{1}{2} |\text{Det}|$

Box volume $= |\mathbf{A} \cdot (\mathbf{B} \times \mathbf{C})| = |\text{Determinant}|$

Equations and Their Solutions

$$y' = cy \quad y_0 e^{ct}$$

$$y' = cy + s \quad y_0 e^{ct} + \frac{s}{c}(e^{ct} - 1)$$

$$y' = cy - by^2 \quad \frac{c}{b+de^{-ct}} \quad d = \frac{c-by_0}{y_0}$$

$$y'' = -\lambda^2 y \quad \cos \lambda t \text{ and } \sin \lambda t$$

$$my'' + dy' + ky = 0 \quad e^{\lambda_1 t} \text{ and } e^{\lambda_2 t} \text{ or } te^{\lambda_1 t}$$

$$y_{n+1} = ay_n \quad a^n y_0$$

$$y_{n+1} = ay_n + s \quad a^n y_0 + s \frac{a^n - 1}{a - 1}$$

Matrices and Inverses

$Ax = \text{combination of columns} = b$

Solution $x = A^{-1}b$ if $A^{-1}A = I$

Least squares $A^T A \bar{x} = A^T b$

$Ax = \lambda x$ (λ is an eigenvalue)

$$\begin{bmatrix} a & b \\ c & d \end{bmatrix}^{-1} = \frac{1}{ad-bc} \begin{bmatrix} d & -b \\ -c & a \end{bmatrix}$$

$$(AB)^{-1} = B^{-1}A^{-1}, (AB)^T = B^T A^T$$

$$\begin{bmatrix} a & b & c \end{bmatrix}^{-1} = \frac{1}{D} \begin{bmatrix} \mathbf{b} \times \mathbf{c} \\ \mathbf{c} \times \mathbf{a} \\ \mathbf{a} \times \mathbf{b} \end{bmatrix}$$

$$\begin{vmatrix} a_1 & a_2 & a_3 \\ b_1 & b_2 & b_3 \\ c_1 & c_2 & c_3 \end{vmatrix} = \begin{vmatrix} +a_1 b_2 c_3 & +a_2 b_3 c_1 & +a_3 b_1 c_2 \\ -a_1 b_3 c_2 & -a_2 b_1 c_3 & -a_3 b_2 c_1 \end{vmatrix}$$

	SI Units	Symbols	From	To	Multiply by
length	meter	m	degrees	radians	.01745
mass	kilogram	kg	calories	joules	4.1868
time	second	s	BTU	joules	1055.1
current	ampere	A	foot-pounds	joules	1.3558
frequency	hertz	Hz $\sim 1/s$	feet	meters	.3048
force	newton	N $\sim \text{kg} \cdot \text{m}/\text{s}^2$	miles	km	1.609
pressure	pascal	Pa $\sim \text{N}/\text{m}^2$	feet/sec	km/hr	1.0973
energy, work	joule	J $\sim \text{N} \cdot \text{m}$	pounds	kg	.45359
power	watt	W $\sim \text{J}/\text{s}$	ounces	kg	.02835
charge	coulomb	C $\sim \text{A} \cdot \text{s}$	gallons	liters	3.785
temperature	kelvin	K	horsepower	watts	745.7
Speed of light	$c = 2.9979 \times 10^8 \text{ m/s}$		Radius at Equator	$R = 6378 \text{ km} = 3964 \text{ miles}$	
Gravity	$G = 6.6720 \times 10^{-11} \text{ Nm}^2/\text{kg}^2$		Acceleration	$g = 9.8067 \text{ m/s}^2 = 32.174 \text{ ft/s}^2$	

Trigonometric Identities

$$\begin{aligned}\sin^2 x + \cos^2 x &= 1 \\ \tan^2 x + 1 &= \sec^2 x \text{ (divide by } \cos^2 x) \\ 1 + \cot^2 x &= \csc^2 x \text{ (divide by } \sin^2 x) \\ \sin 2x &= 2 \sin x \cos x \text{ (double angle)} \\ \cos 2x &= \cos^2 x - \sin^2 x = 2 \cos^2 x - 1 = 1 - 2 \sin^2 x \\ \sin(s \pm t) &= \sin s \cos t \pm \cos s \sin t \text{ (Addition)} \\ \cos(s \pm t) &= \cos s \cos t \mp \sin s \sin t \text{ formulas)} \\ \tan(s + t) &= (\tan s + \tan t) / (1 - \tan s \tan t) \\ c^2 &= a^2 + b^2 - 2ab \cos \theta \text{ (Law of cosines)} \\ a / \sin A &= b / \sin B = c / \sin C \text{ (Law of sines)} \\ a \cos \theta + b \sin \theta &= \sqrt{a^2 + b^2} \cos(\theta - \tan^{-1} \frac{b}{a}) \\ \cos(-x) &= \cos x \text{ and } \sin(-x) = -\sin x \\ \sin(\frac{\pi}{2} \pm x) &= \cos x \text{ and } \cos(\frac{\pi}{2} \pm x) = \mp \sin x \\ \sin(\pi \pm x) &= \mp \sin x \text{ and } \cos(\pi \pm x) = -\cos x\end{aligned}$$

Trigonometric Integrals

$$\begin{aligned}\int \sin^2 x \, dx &= \frac{x - \sin x \cos x}{2} = \int \frac{1 - \cos 2x}{2} \, dx = \frac{x}{2} - \frac{\sin 2x}{4} \\ \int \cos^2 x \, dx &= \frac{x + \sin x \cos x}{2} = \int \frac{1 + \cos 2x}{2} \, dx = \frac{x}{2} + \frac{\sin 2x}{4} \\ \int \tan^2 x \, dx &= \tan x - x \\ \int \cot^2 x \, dx &= -\cot x - x \\ \int \sin^n x \, dx &= -\frac{\sin^{n-1} x \cos x}{n} + \frac{n-1}{n} \int \sin^{n-2} x \, dx \\ \int \cos^n x \, dx &= +\frac{\cos^{n-1} x \sin x}{n} + \frac{n-1}{n} \int \cos^{n-2} x \, dx \\ \int \tan^n x \, dx &= \frac{\tan^{n-1} x}{n-1} - \int \tan^{n-2} x \, dx \\ \int \sec^n x \, dx &= \frac{\sec^{n-2} x \tan x}{n-1} + \frac{n-2}{n-1} \int \sec^{n-2} x \, dx \\ \int \tan x \, dx &= -\ln |\cos x| \\ \int \cot x \, dx &= \ln |\sin x| \\ \int \sec x \, dx &= \ln |\sec x + \tan x| \\ \int \csc x \, dx &= \ln |\csc x - \cot x| = -\ln |\csc x + \cot x| \\ \int \sec^3 x \, dx &= \frac{1}{2} \sec x \tan x + \frac{1}{2} \ln |\sec x + \tan x| \\ \int \sin px \sin qx \, dx &= \frac{\sin(p-q)x}{2(p-q)} - \frac{\sin(p+q)x}{2(p+q)} \\ \int \cos px \cos qx \, dx &= \frac{\sin(p-q)x}{2(p-q)} + \frac{\sin(p+q)x}{2(p+q)} \\ \int \sin px \cos qx \, dx &= -\frac{\cos(p-q)x}{2(p-q)} - \frac{\cos(p+q)x}{2(p+q)}\end{aligned}$$

Additional integrals follow the index

Integration by Parts

$$\begin{aligned}\int \ln x \, dx &= x \ln x - x \\ \int x^n \ln x \, dx &= \frac{x^{n+1} \ln x}{n+1} - \frac{x^{n+1}}{(n+1)^2} \\ \int x^n e^x \, dx &= x^n e^x - n \int x^{n-1} e^x \, dx \\ \int e^{cx} \sin kx \, dx &= \frac{e^{cx}}{c^2 + k^2} (c \sin kx - k \cos kx) \\ \int e^{cx} \cos kx \, dx &= \frac{e^{cx}}{c^2 + k^2} (c \cos kx + k \sin kx) \\ \int x \sin x \, dx &= \sin x - x \cos x \\ \int x \cos x \, dx &= \cos x + x \sin x \\ \int x^n \sin x \, dx &= -x^n \cos x + n \int x^{n-1} \cos x \, dx \\ \int x^n \cos x \, dx &= +x^n \sin x - n \int x^{n-1} \sin x \, dx \\ \int \sin^{-1} x \, dx &= x \sin^{-1} x + \sqrt{1-x^2} \\ \int \tan^{-1} x \, dx &= x \tan^{-1} x - \frac{1}{2} \ln(1+x^2)\end{aligned}$$

Integrals with x^2 and a^2 and $D = b^2 - 4ac$

$$\begin{aligned}\int \frac{dx}{x^2 + a^2} &= \frac{1}{a} \tan^{-1} \frac{x}{a} \\ \int \frac{dx}{a^2 - x^2} &= \frac{1}{2a} \ln \left| \frac{x+a}{x-a} \right| = \frac{1}{a} \tanh^{-1} \frac{x}{a} \\ \int \frac{dx}{\sqrt{x^2 + a^2}} &= \ln |x + \sqrt{x^2 + a^2}| \\ \int \frac{dx}{\sqrt{a^2 - x^2}} &= \sin^{-1} \frac{x}{a} \\ \int \sqrt{x^2 + a^2} \, dx &= \frac{x}{2} \sqrt{x^2 + a^2} + \frac{a^2}{2} \ln |x + \sqrt{x^2 + a^2}| \\ \int \sqrt{a^2 - x^2} \, dx &= \frac{x}{2} \sqrt{a^2 - x^2} + \frac{a^2}{2} \sin^{-1} \frac{x}{a} \\ \int \frac{dx}{x\sqrt{x^2 - a^2}} &= \frac{1}{a} \cos^{-1} \frac{a}{x} \\ \int \frac{dx}{x\sqrt{x^2 + a^2}} &= \frac{1}{a} \ln \left| \frac{\sqrt{x^2 + a^2} - a}{x} \right| \\ \int \frac{dx}{ax^2 + bx + c} &= \frac{1}{\sqrt{D}} \ln \left| \frac{2ax + b - \sqrt{D}}{2ax + b + \sqrt{D}} \right|, D > 0 \\ &= \frac{2}{\sqrt{-D}} \tan^{-1} \frac{2ax + b}{\sqrt{-D}}, D < 0 \\ &= \frac{-2}{2ax + b}, D = 0 \\ \int \frac{dx}{\sqrt{ax^2 + bx + c}} &= \frac{1}{\sqrt{a}} \ln |2ax + b + 2\sqrt{a}\sqrt{ax^2 + bx + c}| \\ &= \frac{1}{\sqrt{-a}} \sin^{-1} \frac{-2ax - b}{\sqrt{-D}}, a < 0\end{aligned}$$

Definite Integrals

$$\begin{aligned}\int_0^\infty x^n e^{-x} \, dx &= n! = \Gamma(n+1) \\ \int_0^\infty e^{-a^2 x^2} \, dx &= \sqrt{\pi}/2a \\ \int_0^1 x^m (1-x)^n \, dx &= \frac{m!n!}{(m+n+1)!} \\ \int_0^\infty \frac{\sin^2 x}{x^2} \, dx &= \int_0^\infty \frac{\sin x}{x} \, dx = \frac{\pi}{2} \\ \int_0^{\pi/2} \sin^n x \, dx &= \int_0^{\pi/2} \cos^n x \, dx = \\ \frac{1}{2} \frac{3}{4} \dots \frac{n-1}{n} \left(\frac{\pi}{2} \right) &\quad \text{or} \quad \frac{2}{3} \frac{4}{5} \dots \frac{n-1}{n} \\ n \text{ even} &\quad \quad \quad n \text{ odd} > 1\end{aligned}$$